Instances/Examples/VexMovRcxRdiFixture.lean
@@ -1,4 +1,4 @@
-import Instances.ISAs.VexISA
+import Instances.ISAs.VexAmd64
 
 set_option autoImplicit false
 set_option relaxedAutoImplicit false
@@ -9,25 +9,26 @@ open VexISA
 
 def bytes : List UInt8 := [0x48, 0x89, 0xf9]
 
-def block : Block :=
-  { stmts := [
+def block : Amd64Block :=
+  mkAmd64Block [
       .wrTmp 0 (.get .rdi),
       .put .rcx (.tmp 0)
-    ],
-    next := 0x400003 }
+    ] 0x400003
 
-def input : ConcreteState :=
-  { rax := 0x0,
-    rcx := 0x0,
-    rdi := 0x10,
-    rip := 0x400000,
-    mem := ByteMem.empty }
+def input : Amd64ConcreteState :=
+  mkAmd64State
+    0x0
+    0x0
+    0x10
+    0x400000
+    ByteMem.empty
 
-def expected : ConcreteState :=
-  { rax := 0x0,
-    rcx := 0x10,
-    rdi := 0x10,
-    rip := 0x400003,
-    mem := ByteMem.empty }
+def expected : Amd64ConcreteState :=
+  mkAmd64State
+    0x0
+    0x10
+    0x10
+    0x400003
+    ByteMem.empty
 
 end Instances.Examples.VexMovRcxRdiFixture
